src/Morph.v
@@ -22,7 +22,8 @@ Open Scope nat_scope.
     states.  It is a [PreOrder] relation. *)
 
 Record SSMorph (sd1 sd2 : ScanStateDesc maxReg) : Prop := {
-    next_interval_increases : nextInterval sd1 <= nextInterval sd2
+    next_interval_increases : nextInterval sd1 <= nextInterval sd2;
+    fixed_intervals_unchanged : fixedIntervals sd1 = fixedIntervals sd2
 }.
 
 Arguments next_interval_increases [sd1 sd2] _.
@@ -32,6 +33,7 @@ Obligation 1. constructor; auto. Qed.
 Obligation 2.
   constructor; destruct H; destruct H0.
   - exact: (leq_trans next_interval_increases0).
+  - by transitivity (fixedIntervals y).
 Qed.
 
 Record SSMorphLen (sd1 sd2 : ScanStateDesc maxReg) : Prop := {
@@ -252,9 +254,10 @@ Defined.
 
 Definition moveActiveToHandled
   `(st : ScanState InUse sd) (spilled : bool) `(H: x \in active sd)
-  (Hreq : if spilled
-          then firstUseReqReg (getInterval (fst x)) == None
-          else true) :
+  (Hreq : let int := vnth (intervals sd) (fst x) in
+          if spilled
+          then firstUseReqReg int.2 == Nothing
+          else verifyNewHandled sd int.1 (snd x)) :
   { sd' : ScanStateDesc maxReg
   | ScanState InUse sd'
   & SSMorphLen sd sd' /\
@@ -303,9 +306,10 @@ Proof. reflexivity. Qed.
 
 Definition moveInactiveToHandled `(st : ScanState InUse sd)
   (spilled : bool) `(H : x \in inactive sd)
-  (Hreq : if spilled
-          then firstUseReqReg (getInterval (fst x)) == None
-          else true) :
+  (Hreq : let int := vnth (intervals sd) (fst x) in
+          if spilled
+          then firstUseReqReg int.2 == Nothing
+          else verifyNewHandled sd int.1 (snd x)) :
   { sd' : ScanStateDesc maxReg
   | ScanState InUse sd'
   & SSMorphLen sd sd' /\
